theories/logatom/rdcss/spec.v
@@ -1,7 +1,7 @@
 From stdpp Require Import namespaces.
 From iris.heap_lang Require Export lifting notation.
 From iris.program_logic Require Export atomic.
-From iris_examples.logatom.rdcss Require Export gc.
+From iris_examples.logatom.lib Require Export gc.
 Set Default Proof Using "Type".
 
 (** A general logically atomic interface for conditional increment. *)
@@ -27,8 +27,8 @@ Record atomic_rdcss {Σ} `{!heapG Σ, !gcG Σ} := AtomicRdcss {
     {{{ True }}}
         new_rdcss #()
     {{{ lln γ, RET lln ; is_rdcss N γ lln ∗ rdcss_content γ 0 }}};
-  rdcss_spec N γ v lm (m1 n1 n2 : Z):
-    is_rdcss N γ v -∗ is_gc_loc lm -∗
+  rdcss_spec N γ v (lm : loc) (m1 n1 n2 : Z):
+    is_rdcss N γ v -∗
     <<< ∀ (m n: Z), gc_mapsto lm #m ∗ rdcss_content γ n >>>
         rdcss #lm v #m1 #n1 #n2 @((⊤∖↑N)∖↑gcN)
     <<< gc_mapsto lm #m ∗ rdcss_content γ (if decide (m = m1 ∧ n = n1) then n2 else n), RET #n >>>;
